NBE.lean
@@ -3,4 +3,5 @@
 import NBE.Kripke
 import NBE.SingleSortImp.Term
 import NBE.SingleSortImp.Beta
+import NBE.SingleSortImp.BetaNormalizing
 import NBE.SingleSortBetaEta
