NBE/SingleSortImp/BetaNormalizing.lean
@@ -1,0 +1,361 @@
+import NBE.SingleSortImp.Beta
+import NBE.SingleSortImp.Presheaf
+
+
+namespace SingleSortImp
+
+namespace BetaNormalizing
+
+def BNE: Presheaf where
+  Pred Γ t T := Γ.Typing t T ∧ exists t', t.beta_eq t' ∧ t'.BNE
+  weaken {Γ' Γ t T} := by
+    intro ⟨HT, t', E, B⟩
+    and_intros
+    . apply Context.weaken_app
+      exact HT
+    . exists t'.up 0 Γ'.length
+      and_intros
+      . apply E.up
+      . exact B.up
+
+
+def BNF: Presheaf where
+  Pred Γ t T := Γ.Typing t T ∧ exists t', t.beta_eq t' ∧ t'.BNF
+  weaken {Γ' Γ t T} := by
+    intro ⟨HT, t', E, B⟩
+    and_intros
+    . apply Context.weaken_app
+      exact HT
+    . exists t'.up 0 Γ'.length
+      and_intros
+      . apply E.up
+      . exact B.up
+
+
+instance: BNF.Typing where
+  typing {Γ t T} := by
+    simp [BNF]
+    intro HT
+    intros
+    exact HT
+
+
+theorem abs_up_app_beta_step {t: Tm}:
+  (t.abs.up0.app (.var 0)).beta_step t
+:= by
+  simp [Tm.up0, Tm.up]
+  apply Tm.beta_step.compute Tm.beta_step.appAbs_ssubst
+  simp [Tm.up_ssubst]
+  conv =>
+    rhs
+    rewrite [Tm.ssubst_id t]
+  congr
+  funext n
+  cases n with
+  | zero =>
+    simp [Subst.comp, Subst.step, Tm.ssubst, Subst.up, Subst.id]
+  | succ =>
+    simp [Subst.comp, Subst.step, Tm.ssubst, Subst.up, Subst.id]
+
+
+theorem beta_eq_normal_beta_mstep {t n: Tm}:
+  t.beta_eq n -> n.normal -> t.beta_mstep n
+:= by
+  intro S N
+  obtain ⟨s, Hts, Hsn⟩ := Relation.church_rosser Tm.beta_step S
+  have E := N.MNormal Hsn
+  cases E
+  exact Hts
+
+
+theorem beta_mstep_app_var_normal' {t s: Tm}:
+  t.beta_eq t.down0.up0 ->
+  (t.app (.var 0)).beta_mstep s ->
+  s.BNF ->
+  exists t', t.beta_mstep t' ∧ t'.BNF
+:= by
+  intro I S N
+  generalize E: (t.app (.var 0)) = m at S
+  induction S generalizing t with
+  | refl =>
+    rewrite [<-E] at N
+    exists t
+    and_intros
+    . apply RTCl.refl
+    . grind [Tm.BNE, Tm.BNF]
+  | step Hxy Hyz IH =>
+    cases Hxy with
+    | abs =>
+      cases E
+    | app2 =>
+      cases E
+      exists t
+    | app1 S' =>
+      cases E
+      rename_i t'
+      have I: t'.beta_eq t'.down0.up0 := by
+        apply ECl.trans
+        . apply ECl.reverse
+          exact S'
+        apply ECl.trans
+        . apply I
+        apply Tm.beta_eq.up
+        apply Tm.beta_eq.down
+        apply ECl.inclusion
+        exact S'
+      obtain ⟨t'', S'', N⟩ := IH I N (by eq_refl)
+      exists t''
+      and_intros
+      . apply RTCl.step
+        . apply S'
+        . apply S''
+      . exact N
+    | appAbs =>
+      cases E
+      rename_i s M
+      have S1: (M.abs.app (.var 0)).beta_eq s := by
+        apply ECl.step
+        . apply Tm.beta_step.appAbs
+        . apply RTCl.sub_ecl
+          exact Hyz
+      have S2: (M.abs.app (.var 0)).beta_eq (M.down 1) := by
+        -- we first change the left to `M.abs.down0.up0`
+        apply ECl.trans
+        . apply Tm.beta_eq.app1
+          exact I
+        simp [Tm.down0, Tm.down]
+        apply ECl.step
+        . apply abs_up_app_beta_step
+        apply ECl.refl
+
+      have S3: M.abs.down0.beta_eq s.abs := by
+        simp [Tm.down0, Tm.down]
+        apply Tm.beta_eq.abs
+        apply ECl.trans
+        . apply ECl.symm
+          exact S2
+        . exact S1
+
+      rewrite [Tm.subst_up_down_var0] at Hyz
+      exists s.abs.up0
+      have N: s.abs.up0.BNF := by
+        apply Tm.BNF.up
+        apply Tm.BNF.abs
+        apply N
+      and_intros
+      . apply beta_eq_normal_beta_mstep _ N.normal
+        apply ECl.trans
+        . exact I
+        apply Tm.beta_eq.up
+        exact S3
+      . exact N
+
+
+theorem beta_eq_app_var_normal {t s: Tm}:
+  ((t.up0.app (.var 0)).beta_eq s) -> s.BNF -> exists t', t.beta_eq t' ∧ t'.BNF
+:= by
+  intro S N
+  replace S := beta_eq_normal_beta_mstep S N.normal
+  have E: t.up0.beta_eq (t.up0.down0.up0) := by simp; apply ECl.refl
+  obtain ⟨s, S, N⟩ := beta_mstep_app_var_normal' E S N
+  exists s.down0
+  and_intros
+  . apply RTCl.sub_ecl
+    apply Tm.beta_mstep.up_down
+    exact S
+  . apply N.down
+
+
+instance BNF.NPair: NPair BNE BNF where
+  atom {Γ t} := by
+    simp [BNE, BNF]
+    grind [Tm.BNE, Tm.BNF]
+
+  imp {Γ Γ'} {t s} {A B} := by
+    rintro ⟨Ht, t', Et', Nt'⟩
+    rintro ⟨Hs, s', Es', Ns'⟩
+    and_intros
+    . constructor
+      . apply Context.weaken_app
+        exact Ht
+      . exact Hs
+    . exists (t'.up 0 Γ'.length).app s'
+      and_intros
+      . apply Tm.beta_eq.app
+        . apply Et'.up
+        . exact Es'
+      . apply Tm.BNE.app
+        . apply Nt'.up
+        . apply Ns'
+  var {Γ A} := by
+    simp [BNE]
+    and_intros
+    . constructor
+      simp
+    . exists (.var 0)
+      and_intros
+      . apply ECl.refl
+      . constructor
+  app_inv {Γ t A B} := by
+    rintro ⟨HT, s, E, N⟩
+    and_intros
+    . cases HT with | app HT1 HT2 =>
+      cases HT2
+      simp_all
+      apply Context.weaken_cons_inv
+      exact HT1
+    . apply beta_eq_app_var_normal
+      . apply E
+      . exact N
+
+
+theorem beta_step_forces {Γ} {t t': Tm} {T}:
+  t.beta_step t' ->
+  BNF.forces Γ t T ->
+  BNF.forces Γ t' T
+:= by
+  intro S F
+  induction T generalizing Γ t t' with
+  | Atom =>
+    simp [Presheaf.forces, forcePred] at *
+    and_intros
+    . apply Tm.beta_step.typing
+      . exact S
+      . apply F.left
+    . obtain ⟨t'', S', N⟩ := F.right
+      exists t''
+      and_intros
+      . apply ECl.trans
+        . symm
+          apply ECl.inclusion
+          exact S
+        . exact S'
+      . exact N
+  | imp T1 T2 IH1 IH2 =>
+    simp [Presheaf.forces, forcePred] at *
+    intro s Γ' F'
+    apply IH2
+    . apply Tm.beta_step.app1
+      apply Tm.beta_step.up
+      exact S
+    . apply F
+      exact F'
+
+
+theorem beta_step_forces' {Γ: Context} {t t': Tm} {T}:
+  Γ.Typing t T ->
+  t.beta_step t' ->
+  BNF.forces Γ t' T ->
+  BNF.forces Γ t T
+:= by
+  intro HT S F
+  induction T generalizing Γ t t' with
+  | Atom =>
+    simp [Presheaf.forces, forcePred] at *
+    and_intros
+    . exact HT
+    . obtain ⟨t'', S', N⟩ := F.right
+      exists t''
+      and_intros
+      . apply ECl.step
+        . exact S
+        . exact S'
+      . exact N
+  | imp T1 T2 IH1 IH2 =>
+    simp [Presheaf.forces, forcePred] at *
+    intro s Γ' F'
+    apply IH2
+    . constructor
+      . apply Context.weaken_app
+        exact HT
+      . replace F' := BNF.NPair.completeness.left F'
+        apply F'.left
+    . apply Tm.beta_step.app1
+      apply Tm.beta_step.up
+      exact S
+    . apply F
+      exact F'
+
+
+theorem beta_mstep_forces' {Γ: Context} {t t': Tm} {T}:
+  Γ.Typing t T ->
+  t.beta_mstep t' ->
+  BNF.forces Γ t' T ->
+  BNF.forces Γ t T
+:= by
+  intro HT S F
+  induction S with
+  | refl =>
+    assumption
+  | step Hxy Hyz IH =>
+    apply beta_step_forces' HT Hxy
+    apply IH (Hxy.typing HT)
+    exact F
+
+
+instance: BNF.MSubst where
+  msubst {Γ t T1 T2 Δ Δ' s env} HT I N F := by
+    apply beta_mstep_forces' _ _ F
+    . -- typing
+      constructor
+      . apply Context.weaken_app
+        apply I.typing
+        constructor
+        exact HT
+      . apply BNF.typing
+        exact N
+    . -- reduction
+      simp [Tm.up, Tm.msubst]
+      apply RTCl.inclusion
+      apply Tm.beta_step.compute
+      apply Tm.beta_step.appAbs_ssubst
+      generalize Δ'.length = n
+      simp [Tm.msubst_ssubst, Tm.up_ssubst]
+      -- we then only have to prove the `Subst`s are the same for those under the length of `var`
+      clear F N
+      apply Tm.ssubst_congr_lt
+      intro x L
+      simp [Subst.comp]
+      cases x with
+      | zero =>
+        simp [Env.subst, Tm.ssubst, Subst.comp, Subst.up, Subst.step]
+      | succ x =>
+        unfold Env.subst
+        replace L: x < env.length := by
+          replace HT := HT.bound
+          simp at HT
+          rewrite [I.length]
+          omega
+        have E {s c n}: Tm.msubst_var (s :: env.up c n) (x + 1) = (env[x]).up c n := by
+            simp [<-Env.up_index_lt]
+            apply Tm.msubst_var_lt
+            simp
+            exact L
+        simp [E]
+        generalize env[x] = env'
+        simp [Tm.up_ssubst]
+        -- again, we only have to prove the beta_eq of the `Subst`
+        clear HT T1 T2 E L x I env Γ
+        congr
+        funext x
+        cases x with
+        | zero =>
+          simp [Tm.ssubst, Subst.up, Subst.comp, Subst.step]
+          grind
+        | succ =>
+          simp [Tm.ssubst, Subst.up, Subst.comp, Subst.step]
+          grind
+
+
+/--
+This is the result of the real completeness
+-/
+theorem beta_step_normalizing {Γ: Context} {t T}:
+  Γ.Typing t T -> exists t', t.beta_eq t' ∧ t'.BNF
+:= by
+  intro HT
+  let entailment := BNF.NPair.soundness HT
+  specialize entailment Γ (Env.vars Γ.length) Instantiate.self
+  simp at entailment
+  let F := BNF.NPair.completeness.left entailment
+  apply F.right
